theories/thunks/ThunksExamples.v
@@ -23,10 +23,10 @@ Implicit Type t : loc.
 
 Lemma create_thunk_forcing_thunk p N1 F2 t2 n2 R φ :
   TC_invariant -∗
-  {{{ TC 3 ∗ Thunk p F2 t2 n2 R φ }}}
+  {{{ TC Tcr ∗ Thunk p F2 t2 n2 R φ }}}
     « create (λ: <>, force #t2)%V »
   {{{ t1, RET «#t1» ;
-      Thunk p (↑N1) t1 (12+n2) (ThunkToken p F2 ∗ R)
+      Thunk p (↑N1) t1 (Tf+1+n2) (ThunkToken p F2 ∗ R)
             (λ v, ThunkVal t2 v ∗ □ φ v)
   }}}.
 Proof.
